SchnorrPK

examples/SchnorrPK.ec
@@ -15,151 +15,87 @@ require import CyclicGroup.
 require (*--*) SigmaProtocol.
 
 (* Schnorr protocol types *)
-theory SchnorrTypes.
-  type statement    = group.
-  type witness      = F.t.
-  type message      = group.
-  type secret       = F.t.
-  type challenge    = F.t.
-  type response     = F.t.
+type statement    = group.
+type witness      = F.t.
+type message      = group.
+type challenge    = F.t.
+type response     = F.t.
 
-  op R_DL h w       = (h = g^w).
-end SchnorrTypes.
-export SchnorrTypes.
+op R (h:statement) (w:witness) = h = g^w.
+op challenges = FDistr.dt.
+
+op verify (h: statement) (a: message) (e: challenge) (z: response) : bool = 
+  a * h^e = g^z.
 
 (* Instantiate the Sigma scheme with the above types *)
-clone import SigmaProtocol as SP with
-  type SigmaProtocol.statement <- statement,
-  type SigmaProtocol.witness   <- witness,
-  type SigmaProtocol.message   <- message,
-  type SigmaProtocol.secret    <- secret,
-  type SigmaProtocol.challenge <- challenge,
-  type SigmaProtocol.response  <- response,
-  op   SigmaProtocol.R         = R_DL,
-  op   SigmaProtocol.de        = FDistr.dt.
-export SigmaProtocol.
+clone include SigmaProtocol.SP with
+  type statement  <- statement,
+  type witness    <- witness,
+  type message    <- message,
+  type challenge  <- challenge,
+  type response   <- response,
+  op   R          <- R,
+  op   challenges <- challenges,
+  op   verify     <- verify
+  proof *.
 
-module SchnorrPK : SigmaScheme = {
-  proc gen() : statement * witness = {
-    var h, w;
-    w =$ FDistr.dt;
-    if (w = F.zero) { (* A loop would be better, however the support for while loops is poor *)
-      w = -F.one;
-    }
-    h = g^w;
-    return (h, w);
+module P : Prover = {
+  proc gen () : statement * witness = {
+    var w;
+    w <$ challenges; 
+    return (g^w, w);
   }
 
-  proc commit(h: statement, w: witness) : message * secret = {
-    var r, a;
-    r =$ FDistr.dt;
-    a = g^r;
-    return (a, r);
+  var w_ : witness
+  var r  : F.t
+  
+  proc init (x:statement, w:witness) : message = {
+    w_ <- w;
+    r  <$ challenges;
+    return g^r;
   }
 
-  proc test(h: statement, a: message) : challenge = {
-    var e;
-    e =$ FDistr.dt;
-    return e;
-  }
-
-  proc respond(sw: statement * witness, ms: message * secret, e: challenge) : response = {
-    var z, w, r;
-    w = snd sw;
-    r = snd ms;
-    z = r + e*w;
-    return z;
-  }
-
-  proc verify(h: statement, a: message, e: challenge, z: response) : bool = {
-    var v, v';
-    v = a*(h^e);
-    v' = g^z;
-    return (v = v');
+  proc respond (e: challenge) : response = {
+    return r + e * w_;
   }
 }.
 
-module SchnorrPKAlgorithms : SigmaAlgorithms = {
-  proc soundness(h: statement, a: message, e: challenge, z: response, e': challenge, z': response) : witness option = {
-    var sto, w, v, v';
-
-    v  = (g^z  = a*(h^e ));
-    v' = (g^z' = a*(h^e'));
-    if (e <> e' /\ v /\ v') {
-      w = (z - z') / (e - e');
-      sto = Some(w);
-    } else {
-      sto = None;
-    }
-
-    return sto;
-  }
-
-  proc simulate(h: statement, e: challenge) : message * challenge * response = {
-    var a, z;
-
-    z  =$ FDistr.dt;
-    a  = (g^z) * (h^(-e));
-
-    return (a, e, z);
+module KE: KnowledgeExtractor = {
+  proc extract(x: statement, a: message, e: challenge, z: response, e': challenge, z': response) : witness = {
+    return  (z - z') / (e - e');
   }
 }.
 
-section SchnorrPKSecurity.
-  (* Completeness *)
-  lemma schnorr_proof_of_knowledge_completeness_ll:
-    islossless Completeness(SchnorrPK).main.
-  proof. by islossless; apply FDistr.dt_ll. qed.
+module S:Simulator = { 
+  proc simulate(x: statement, e: challenge) : message * response = {
+    var z;
+    z  <$ FDistr.dt;
+    return (g^z * x^(-e), z);
+  }
+}.
 
-  lemma schnorr_proof_of_knowledge_completeness h w' &m:
-    R h w' =>
-    Pr[Completeness(SchnorrPK).main(h, w') @ &m : res] = 1%r.
-  proof.
-    rewrite /R /R_DL; move => sigmarel.
-    byphoare (_: h = x /\ w' = w ==> _) => //; rewrite sigmarel.
-    proc; inline*; swap 3 -2; swap 8 -7.
-    wp; rewrite /snd /=; auto => &hr />.
-    rewrite FDistr.dt_ll => /> *; algebra.
-  qed.
+lemma Completeness : 
+  phoare [Completeness(P).main : R x w ==> res] = 1%r.
+proof.
+  proc;inline * => /=.
+  conseq (: true ==> true) (: R x w ==> verify x a e z) => //; last by islossless.
+  by auto;rewrite /verify /R => /> *;algebra.
+qed.
 
-  (* Special soundness *)
-  lemma schnorr_proof_of_knowledge_special_soundness (h: statement) msg ch ch' r r' &m:
-    ch <> ch' =>
-    g^r  = msg*(h^ch ) =>
-    g^r' = msg*(h^ch') =>
-    Pr[SpecialSoundnessExperiment(SchnorrPK, SchnorrPKAlgorithms).main(h, msg, ch, r, ch', r') @ &m : (res <> None /\ R h (oget res))] = 1%r.
-  proof.
-    move => challenges_differ
-            accepting_transcript_1
-            accepting_transcript_2.
-    byphoare (_: h = x /\ msg = m /\ ch = e /\ ch' = e' /\ r = z /\ r' = z' ==> _) => //.
-    proc; simplify; inline*.
-    auto; rewrite /R /R_DL /oget => &hr /> ? 2!-> /=.
-    rewrite F.div_def -pow_pow F.sub_def -mul_pow pow_opp log_bij.
-    rewrite accepting_transcript_1 accepting_transcript_2 !(log_gpow, log_pow, log_mul, inv_def). 
-    by field; apply: contra H => heq; ring heq.
-  qed.
+lemma SpecialSoundness :
+  phoare [SpecialSoundness(KE).main : verify x a e z /\ verify x a e' z' /\ e <> e' ==> res] =  1%r.
+proof.
+  proc; inline *; auto; rewrite /verify /R => /> &m.
+  rewrite !(log_bij, log_g, log_pow, log_mul) => h1 h2 he.
+  by field h1 h2; apply /negP => h; apply he; ring h.
+qed.
 
-  (* Special honest verifier zero knowledge *)
-  lemma schnorr_proof_of_knowledge_shvzk (D<: SigmaTraceDistinguisher) &m:
-    Pr[SimulateHonestVerifier(SchnorrPK, SchnorrPKAlgorithms, D).gameIdeal() @ &m : res] = 
-    Pr[SimulateHonestVerifier(SchnorrPK, SchnorrPKAlgorithms, D).gameReal() @ &m : res].
-  proof.
-  (*  move : FDistr.dt_ll FDistr.dt_fu FDistr.dt1E; rewrite /is_full => dt_ll dt_fu dt_supp. *)
-    byequiv => //.
-    proc; inline*.
-    seq 27 22: ((glob D){1} = (glob D){2} /\ i{1} = 0 /\ x{1} = h{1} /\ x{2} = h{2} /\ 
-                 to{1} = Some t{2} /\ ={h, w, e}).
-    + swap{1} 15 -7; swap{2} 12 -5; swap{1} 11 -3; wp.
-      (* Let's play with randomness... *)
-      rnd (fun z, z - w{1}*e{1}) (fun r, r + w{1}*e{1}).
-      by seq 2 2 : (#pre  /\ ={w0}); auto => />; progress;algebra.
-    by call (_:true); rcondf{1} 1; auto.
-  qed.
-  (* The above three theorems prove that the Schnorr proof of knowledge is a Sigma protocol *)
+lemma sHVZK : 
+  equiv [RealP(P).main ~ S.simulate : (R x w) {1} /\ ={x,e} ==> ={res}].
+proof.
+  proc; inline *; wp.
+  rnd (fun r => r + log x{2} * e{2}) (fun r => r + log x{2} * -e{2}) .
+  auto; rewrite /R => /> &1 &2; split; 1: by move=> *;ring.
+  move=> h r hr;split => [ | _];2:split; algebra.
+qed.
 
-end section SchnorrPKSecurity.
-
-print schnorr_proof_of_knowledge_completeness.
-print schnorr_proof_of_knowledge_special_soundness.
-print schnorr_proof_of_knowledge_shvzk.
